wip linear: tuple to thread_t record.

src/spec/Flutterbye.Linearization.fst
@@ -27,6 +27,12 @@ type step_t 'a =
    | Commit: op:('a -> Tot 'a) -> step_t 'a
    | Stale: op:('a -> Tot 'a) -> step_t 'a
 
+type thread_t 'a =
+   {
+      steps:seq (step_t 'a);
+      state:'a;
+   } 
+
 type satisfies_commit_p (#a_t:Type) (steps:seq (step_t a_t)) =
    satisfies_p is_Commit steps
 
@@ -41,11 +47,11 @@ val linearize_inner_induction_loop:
       pending:seq (pending_t 'a)
    -> state:'a
    -> steps:seq (step_t 'a){satisfies_commit_p steps \/ satisfies_fresh_p pending state}
-   -> Tot (out:(seq (step_t 'a) * 'a){satisfies_commit_p (fst out)})
+   -> Tot (thread':(thread_t 'a){satisfies_commit_p thread'.steps})
       (decreases (length pending))
 let rec linearize_inner_induction_loop pending state steps =
    if 0 = length pending then
-      (steps, state)
+      { steps = steps; state = state }
    else begin
       let i = 0 in
       let p = index pending i in
@@ -78,7 +84,7 @@ let rec linearize_inner_induction_loop pending state steps =
 val linearize_inner_induction:
       pending:seq (pending_t 'a)
    -> state:'a{satisfies_fresh_p pending state}
-   -> Tot (out:(seq (step_t 'a) * 'a){satisfies_commit_p (fst out)})
+   -> Tot (thread':(thread_t 'a){satisfies_commit_p thread'.steps})
       (decreases (length pending))
 let linearize_inner_induction pending state =
    linearize_inner_induction_loop pending state createEmpty
